src/ref4/Curve25519_auto4.ec
@@ -1,33 +1,429 @@
-require import Int Bool Zp_25519 List.
+require import Int StdOrder Ring IntDiv Bool Zp_25519 List Real.
 require import Curve25519_Spec.
 require import Curve25519_Hop1.
 require import Curve25519_Hop2.
 require import Curve25519_Ref4.
 require import W64limbs.
+require import StdOrder.
+from Jasmin require import JWord JWord_array JModel JUtils.
 
-from Jasmin require import JWord JWord_array.
+import Zp_25519 Curve25519_Spec Curve25519_Hop2 Curve25519_Ref4 Array4 Array32 Ring.IntID StdOrder.IntOrder Array4.
 
-import Zp_25519 Curve25519_Spec Curve25519_Hop2 Curve25519_Ref4 Array4 Array32.
+op modulus : int = W64.modulus ^ 4.
 
-(* Probably needs to be moved elsewhere, such as W64limbs *)
+lemma modulusE: modulus = W64.modulus ^ 4 by rewrite /modulus.
+
+type limb = W64.t.
+
+
+module GenericOperations = {
+    proc addn(a : int, b : int) : bool * int = {
+        var c : bool;
+        var r : int;
+
+        c <- modulus <= a + b;
+        r <- (a + b) %% modulus;
+
+        return (c, r);
+    }
+    
+    proc maskOnCarry(m: int, r: W64.t, cf: bool): W64.t = {
+        (cf, r) <- subc r r cf;
+        r <- r `&` W64.of_int m;
+        return r;
+    }
+    
+    proc addcR( a b: Rep4, c: bool): bool * Rep4 =     {
+        var r: Rep4;
+        var i, x;
+        r <- witness;
+        i <- 0;
+        while (i < 4) {
+            (c, x) <- addc a.[i] b.[i] c;
+            r.[i] <- x;
+            i <- i + 1;
+        }
+        return (c,r);
+      }
+    
+    
+   proc addcR2( a b: Rep4): bool * Rep4 =     {
+    
+        
+        var i, x, c;
+        c <- false;
+        i <- 0;
+        
+        while (i < 4) {
+            (c, x) <- addc a.[i] b.[i] c;
+            a.[i] <- x;
+            i <- i + 1;
+        }
+        return (c,a);
+    }
+    
+    
+    
+    proc addl (a b: Rep4) : Rep4 = {
+        var h, z0 : Rep4;
+        var z, tt : limb;    
+        var c, t0 : bool;
+        var i : int;
+        h <- a;
+        z <- W64.zero;
+        
+        (c, h) <@ addcR2(h, b);
+         z <@ maskOnCarry(38, z, c);
+         
+        z0.[0] <- z;
+        z0.[1] <- W64.zero;
+        z0.[2] <- W64.zero;
+        z0.[3] <- W64.zero;
+        
+        (c, h) <@ addcR2(h, z0);
+        z <@ maskOnCarry(38, z, c);
+        h.[0] <- h.[0] + z;  
+
+    return h;
+    }
+
+}.
+
+
+equiv eq_h4_add_rrs_proc : M_ref4.__add4_rrs ~ GenericOperations.addl:
+   f{1}   =  a{2} /\
+   g{1}   =  b{2}
+   ==> 
+   res{1} = res{2}. 
+proof.
+    proc. inline *. do 2! unroll for{2} ^while. do 2! unroll for{1} ^while.   
+    wp. skip => />. 
+qed.
+
 
 (** step 0 : add sub mul sqr - all done by auto **)
 
-equiv eq_h4_add_rrs_ref4 : MHop2.add ~ M_ref4.__add4_rrs:
-    f{1}   = inzpRep4 f{2} /\
-    g{1}   = inzpRep4 g{2}
-    ==>
-    res{1} = inzpRep4 res{2}.
+lemma lex_lt x1 x2 m y1 y2:
+ 0 < m => 0 <= x1 < m => 0 <= x2 < m => 0 <= y1 => 0 <= y2 =>
+ (y1*m + x1 < y2*m + x2) = (y1 < y2 \/ y1=y2 /\ x1 < x2)
+by smt().
+(*proof. by move=> /> *; rewrite (divzU (y1 * m + x1) m y1 x1) /#. qed.*)
+
+lemma lex_le x1 x2 m y1 y2:
+ 0 < m => 0 <= x1 < m => 0 <= x2 < m => 0 <= y1 => 0 <= y2 =>
+ (y1*m + x1 <= y2*m + x2) = (y1 < y2 \/ y1=y2 /\ x1 <= x2)
+by smt().
+(*proof. by move=> /> *; rewrite (divzU (y1 * m + x1) m y1 x1) /#. qed.*)
+
+lemma lex_eq x1 x2 m y1 y2:
+ 0 < m => 0 <= x1 < m => 0 <= x2 < m => 0 <= y1 => 0 <= y2 =>
+ (y1*m + x1 = y2*m + x2) = (y1 = y2 /\ x1 = x2)
+by smt().
+
+lemma modz_pow (a b d: int):
+ 0 <= b => a ^ b %% d = (a %% d) ^ b %% d.
+proof.
+elim/natind: b.
+ by move => n *; rewrite (_:n=0) 1:/# !expr0.
+move=> n Hn IH H.
+rewrite !exprS 1..2://.
+by rewrite eq_sym -modzMmr -IH 1:// modzMmr modzMml.
+qed.
+
+
+lemma addcP' (x y: limb, c :  bool):
+    to_uint (W64.addc x y c).`2 = to_uint x + to_uint y + b2i c - b2i (carry_add x y c) * W64.modulus.
+proof.
+rewrite addcE /= /carry_add.
+case: (W64.modulus <= to_uint x + to_uint y + b2i c) => E.
+ rewrite to_uintD of_uintK b2i1 /= (modz_small (b2i c)); first smt(ge2_modulus).
+ rewrite to_uintD modzDml -(modzMDr (-1)) modz_small //=.
+ case: c E; rewrite /b2i /=; move: W64.to_uint_cmp; smt(). rewrite !b2i0 => />.  
+smt(W64.to_uintD_small W64.of_uintK modz_small W64.to_uint_cmp ge2_modulus bound_abs).
+qed.
+
+lemma addcPP (a b: limb, c: bool):
+    to_uint (W64.addc a b c).`2 = to_uint a + to_uint b + b2i c - b2i (W64.addc a b c).`1 * W64.modulus.
+proof.
+    by rewrite addcP' /addc /= /carry_add.
+qed.
+
+
+op dig (x: Rep4) (i:int): int = to_uint x.[i]*W64.modulus^i.
+
+lemma digE (x: Rep4) (i:int): dig x i = to_uint x.[i]*W64.modulus^i by rewrite /dig.
+hint simplify digE.
+
+(* BigInt value for a prefix of an array *)
+op valRep4_partial (k:int) (x:Rep4): int = 
+    foldr Int.(+) 0 (map (dig x) (range 0 k)).
+
+op valRep4_full (x : Rep4) : int = 
+    valRep4_partial 4 x.
+
+lemma eq_valRep4_full (x : Rep4):
+     valRep4_full x = valRep4 x.
+proof.
+    by rewrite /valRep4_full valRep4E /val_digits /valRep4_partial  /range /to_list /mkseq -iotaredE => />; ring.
+qed.
+
+lemma valRep4_partialN (k: int,  x : Rep4): 
+    k <= 0 => valRep4_partial k x = 0.
 proof. 
-    proc.  
-    admit.
+    move => ?; rewrite /valRep4_partial /range -iotaredE => />. smt(@List). 
+qed.
+
+lemma valRep4_partial0 (x: Rep4): 
+    valRep4_partial 0 x = 0.
+proof. 
+    by rewrite valRep4_partialN. 
+qed.
+
+(* less generic, but we only care about 4 limbs *)
+lemma valRep4_partialS (k: int, x : Rep4): 
+    0 <= k <= 4 => valRep4_partial (k+1) x = dig x k + valRep4_partial k x.
+proof. 
+    case: (k=0) => E.
+    + by rewrite E /= /valRep4_partial rangeS range_geq 1://. 
+    case: (k=1) => E0.
+    rewrite E0 /= /valRep4_partial /range -iotaredE => />. ring. 
+    case: (k=2) => E1.
+    rewrite E1 /= /valRep4_partial /range -iotaredE => />. ring. 
+    case: (k=3) => E2.
+    rewrite E2 /= /valRep4_partial /range -iotaredE => />. ring.
+    case: (k=4) => E3.
+    rewrite E3 /= /valRep4_partial /range -iotaredE => />. ring.
+    auto => />. smt().
+qed.
+
+lemma valRep4_partial1 x: 
+    valRep4_partial 1 x = dig x 0.
+proof. 
+    by rewrite -(add0z 1) valRep4_partialS 1:/# digE expr0 valRep4_partial0. 
+qed.
+
+
+lemma valRep4_partial_cmp (k : int,  x : Rep4): 0 <= k <= 4 =>  0 <= valRep4_partial k x < W64.modulus^k.
+proof.
+    case: (k=0) => E.
+        + rewrite E valRep4_partial0 !expr0. smt().
+    case: (k=1) => E1.
+        + rewrite E1. rewrite /valRep4_partial /range -iotaredE => />. split. smt(W64.to_uint_cmp).
+        + move => H. move: W64.to_uint_cmp x.[0]  => />. move => H0. smt().
+    case: (k=2) => E2.
+        + rewrite E2. rewrite /valRep4_partial /range -iotaredE => />. split. smt(W64.to_uint_cmp).
+        + move => H. smt(@W64 @JUtils).
+    case: (k=3) => E3.
+        + rewrite E3. rewrite /valRep4_partial /range -iotaredE => />. split. smt(W64.to_uint_cmp).
+        + move => H. smt(@W64 @JUtils).
+    case: (k=4) => E4.
+        + rewrite E4. rewrite /valRep4_partial /range -iotaredE => />. split. smt(W64.to_uint_cmp).
+        + move => H. smt(@W64 @JUtils).
+    auto => />. smt().
+qed.
+
+lemma valRep4_partial_ltb (k : int,  x y : Rep4,  b : bool):
+    0 <= k <= 4 => valRep4_partial (k+1) x < valRep4_partial (k+1) y + b2i b
+    = (to_uint x.[k] < to_uint y.[k] \/ x.[k]=y.[k] /\ 
+      valRep4_partial k x < valRep4_partial k y + b2i b).
+proof.
+    move=> [?] ?; rewrite !valRep4_partialS // !digE.
+    move: (W64.to_uint_cmp x.[k]) (W64.to_uint_cmp y.[k]) =>  *.
+    case: b => E; rewrite ?b2i1 ?b2i0 => *.
+    rewrite !ltzS lex_le ?expr_gt0 //; move: valRep4_partial_cmp W64.to_uint_eq; smt().
+    by rewrite /= lex_lt ?expr_gt0 //; move: valRep4_partial_cmp W64.to_uint_eq; smt().
+qed.
+
+lemma valRep4_partial_setO k x i y:
+    0 <= k <= i < 4 => valRep4_partial k x.[i <- y]%Array4 = valRep4_partial k x.
+proof.
+    elim/natind: k => /=.
+    by move=> k *; rewrite (_:k=0) 1:/# !valRep4_partial0.
+    move=> k Hk IH H; rewrite !valRep4_partialS //. smt(). smt(). rewrite !digE !get_setE 1:/# IH /#.
+qed.
+
+
+op carry_add_on_k (k : int, x y: Rep4, c:bool): bool =
+    iteri k (fun i r => carry_add x.[i] y.[i] r) c.
+
+lemma carry_add_on_k0 (x y: Rep4 , c: bool) : carry_add_on_k 0 x y c = c by rewrite /carry_add_on_k iteri0.
+
+lemma carry_add_on_kS (k : int, x y: Rep4, c:bool):
+    0 <= k => carry_add_on_k (k+1) x y c = (carry_add x.[k] y.[k] (carry_add_on_k k x y c)) 
+        by move=> *; rewrite /carry_add_on_k iteriS.
+
+lemma carry_add_on_kP (k : int, x y: Rep4, c:bool):
+    0 <= k <= 4 =>
+    b2i (carry_add_on_k k x y c) = (valRep4_partial k x + valRep4_partial k y + b2i c) %/ W64.modulus^k.
+proof.
+    move => [H] H0.
+    case: (k = 0) => H1.
+    rewrite /carry_add_on_k H1 !valRep4_partial0 iteri0 => />.
+    case: (k = 1) => H2.
+    rewrite /carry_add_on_k H2 !valRep4_partial1 iteri_red // iteri0 // !digE => />.
+    rewrite /carry_add. 
+    case (W64.modulus <= to_uint x.[0] + to_uint y.[0] + b2i c) => H3. 
+    rewrite b2i1 => />. smt(@W64 @JUtils).
+    rewrite b2i0 => />. smt(@W64 @JUtils).
+    case: (k = 2) => H3.
+    rewrite /carry_add_on_k H3 !/valRep4_partial iteri_red  // iteri_red => />.
+    rewrite iteri0 // /range -iotaredE => />. 
+    case (carry_add x.[1] y.[1] (carry_add x.[0] y.[0] c)) => H4.
+    rewrite b2i1 => />. smt(@W64 @JUtils).
+    rewrite b2i0 => />. smt(@W64 @JUtils).
+    case: (k = 3) => H4.
+    rewrite /carry_add_on_k H4 !/valRep4_partial iteri_red // iteri_red // iteri_red => />.
+    rewrite iteri0 // /range -iotaredE => />. 
+    case (carry_add x.[2] y.[2] (carry_add x.[1] y.[1] (carry_add x.[0] y.[0] c))) => H5.
+    rewrite b2i1 => />. smt(@W64 @JUtils).
+    rewrite b2i0 => />. smt(@W64 @JUtils).
+    case: (k = 4) => H5.
+    rewrite /carry_add_on_k H5 !/valRep4_partial iteri_red // iteri_red // iteri_red // iteri_red => />.
+    rewrite iteri0 // /range -iotaredE => />. 
+    case (carry_add x.[3] y.[3] (carry_add x.[2] y.[2] (carry_add x.[1] y.[1] (carry_add x.[0] y.[0] c)))) => H6.
+    rewrite b2i1 => />. smt(@W64 @JUtils).
+    rewrite b2i0 => />. smt(@W64 @JUtils).
+    auto => />. smt(). 
+qed.
+
+lemma carry_add_on_kE (k : int,  x y : Rep4, c : bool):
+    0 <= k <= 4 => carry_add_on_k k x y c = (W64.modulus^k <= valRep4_partial k x + valRep4_partial k y + b2i c).
+proof.
+    move => [H] H0.
+    case: (k = 0) => H1.
+    rewrite H1 /carry_add_on_k !valRep4_partial0 iteri0 // => />. smt().
+    case (k = 1) => H2.
+    rewrite H2 /carry_add_on_k /valRep4_partial /range -iotaredE iteri_red // iteri0 //.
+    case (k = 2) => H3.
+    rewrite H3 /carry_add_on_k /valRep4_partial /range -iotaredE iteri_red // iteri_red //  iteri0 // => />.
+    case (carry_add x.[1] y.[1] (carry_add x.[0] y.[0] c)) => H4.
+    smt(@W64 @JUtils). smt(@W64 @JUtils).
+    case (k = 3) => H4.
+    rewrite H4 /carry_add_on_k /valRep4_partial /range -iotaredE iteri_red // iteri_red // iteri_red // iteri0 // => />.
+    case (carry_add x.[2] y.[2] (carry_add x.[1] y.[1] (carry_add x.[0] y.[0] c))) => H5.
+    smt(@W64 @JUtils). smt(@W64 @JUtils).
+    case (k = 4) => H5.
+    rewrite H5 /carry_add_on_k /valRep4_partial /range -iotaredE iteri_red // iteri_red // iteri_red  // iteri_red // iteri0 // => />.
+    case (carry_add x.[3] y.[3] (carry_add x.[2] y.[2] (carry_add x.[1] y.[1] (carry_add x.[0] y.[0] c)))) => H6.
+    smt(@W64 @JUtils). smt(@W64 @JUtils).
+    auto => />. smt().
+qed.
+
+
+lemma addcR_h aa bb cc:
+  hoare [ GenericOperations.addcR:
+          aa = a /\ bb = b /\ cc = c
+          ==>
+          res.`1 = modulus <=  valRep4_full aa + valRep4_full bb +  b2i cc
+          /\ valRep4_full res.`2 = ( valRep4_full aa + valRep4_full  bb + b2i cc) %% modulus
+        ].
+proof.
+    proc => /=.
+    while (0 <= i <= 4 /\ a = aa /\ b = bb /\
+        c = carry_add_on_k i aa bb cc /\
+        valRep4_partial i r = valRep4_partial i aa + valRep4_partial i bb + b2i cc - b2i c * W64.modulus^i
+    ).
+    wp. skip => &hr [[[H H0]]] /> H1 H2.
+    split; first smt().
+    split.
+    rewrite addcE !carry_add_on_kS /= // /carry_add.    
+    rewrite !valRep4_partialS // !digE get_setE //= valRep4_partial_setO 1:/# H1.
+    by rewrite addcP' !exprS // !/carry_add_on_k addcE !/carry_add /=; ring.
+    wp; skip => />; auto => />.
+    do split.
+    + by rewrite carry_add_on_k0.
+    + by rewrite !valRep4_partial0 // expr0 /#.
+    move => H H0  H1  H2 H3 H5. split.
+   
+    move: valRep4_partial_cmp. smt(@JUtils).
+    move: valRep4_partial_cmp. smt(@JUtils).
+qed.
+
+lemma addcR_ll: islossless GenericOperations.addcR.
+proof.
+    proc. unroll for ^while.
+    islossless.
+qed.
+
+lemma addcR_ph aa bb cc:
+ phoare [ GenericOperations.addcR:
+          aa = a /\ bb = b /\ cc = c
+          ==>
+          res.`1 = modulus <=  valRep4_full aa + valRep4_full bb +  b2i cc
+          /\ valRep4_full res.`2 = ( valRep4_full aa + valRep4_full  bb + b2i cc) %% modulus
+        ] = 1%r.
+proof. by conseq addcR_ll (addcR_h aa bb cc). qed.
+
+equiv addc_spec:
+ GenericOperations.addcR2 ~ GenericOperations.addn:
+  valRep4_full a{1} = a{2} /\ valRep4_full b{1} =  b{2}
+  ==> res{1}.`1=res{2}.`1 /\ valRep4_full res{1}.`2 =  res{2}.`2.
+proof.
+    transitivity 
+     GenericOperations.addcR
+     ( ={a,b} /\ !c{2} ==> ={res} )
+     ( valRep4_full a{1} =  a{2} /\ valRep4_full b{1} =  b{2} /\ !c{1}
+       ==> res{1}.`1 = res{2}.`1 /\ valRep4_full res{1}.`2 = res{2}.`2 ).
+    + by move=> /> &1 &2 H1 H2; exists (a{1},b{1},false).
+    + by move=> /> *.
+    + proc. simplify.
+    unroll {2} 3; rcondt {2} 3; first by auto.
+    unroll {1} 3; rcondt {1} 3; first by auto.
+    exlim a{1}, b{1} => aa bb.
+    while (={i,b} /\ 1 <= i{2} <= 4 /\
+         (c,aa){1}=(c,a){2} /\rewrite !b2i0 => />. move => T T0 T1. split.
+  rewrite T0 /modulus /=. 
+  rewrite !eq_valRep4_full. 
+  have E: valRep4 a{1} = a{2}. smt.
+  smt.
+    by rewrite carry_add_on_kE 1:/# b2i0 /modulus /=.
+
+         (forall k, 0 <= k < i{2} => a{1}.[k] = r{2}.[k]) /\
+         (forall k, i{2} <= k < 4 => a{1}.[k] = aa.[k])).
+    wp; skip => /> &1 &2 Hi1 Hi2 H1 H2 Hi.
+    split => *; first smt().
+    split => *; first smt().
+    split.
+    move=> k Hk1 Hk2.
+    pose X := (addc _ _ _)%W64.
+    pose Y := (addc _ _ _)%W64.
+    have ->: X=Y by smt().
+    case: (k = i{2}) => ?.
+     by rewrite !set_eqiE /#.
+    by rewrite !set_neqiE /#.
+   move=> k Hk1 Hk2.
+   by rewrite set_neqiE /#.
+   wp. skip => /> &1. 
+   move=> Hc; split => *. 
+   split => k *.
+    by rewrite (_:k=0) 1:/# !set_eqiE /#.
+   by rewrite set_neqiE /#.
+  by apply ext_eq; smt().
++ proc. simplify.
+  transitivity {1}
+   { (c,r) <@ GenericOperations.addcR(a,b,c); }
+   ( ={a,b,c} ==> ={c,r} )
+   (  valRep4_full a{1} = a{2} /\ valRep4_full b{1}=  b{2} /\ !c{1} ==> ={c} /\ valRep4_full r{1} =  r{2} ).
+   by move=> /> &1 &2; exists a{1} b{1} false.
+  + by auto.
+  + by inline *; sim.
+  + ecall {1} (addcR_ph a{1} b{1} c{1}); wp; skip => /> &1 &2 &m H0 Hc  /=.
+qed.
+
+equiv eq_h4_add_rrs_ref4 : MHop2.add ~ M_ref4.__add4_rrs:
+   f{1}   = inzpRep4 f{2} /\
+   g{1}   = inzpRep4 g{2}
+   ==> 
+   res{1} = inzpRep4 res{2}.
+proof.
+    
 qed.
 
 equiv eq_h4_sub_rrs_ref4 : MHop2.sub ~ M_ref4.__sub4_rrs:
    f{1}   = inzpRep4 f{2} /\
    g{1}   = inzpRep4 gs{2}
    ==>
-   res{1} = inzpRep4 res{2}.
+ s  res{1} = inzpRep4 res{2}.
 proof.
     proc *. 
     admit.
@@ -49,8 +445,8 @@ equiv eq_h4_mul_rss_ref4 : MHop2.mul ~ M_ref4.__mul4_rss:
     ==>
     res{1} = inzpRep4 res{2}.
 proof.
-    proc *. 
-    admit.
+   proc.  
+   
 qed.
 
 equiv eq_h4_sqr_ref4 : MHop2.sqr ~ M_ref4.__sqr4_rs:
